Refactored `LowStar.RVector` a lot

ulib/LowStar.RVector.fst
@@ -74,9 +74,11 @@ noeq type regional a =
     r_init: (r:erid ->
       HST.ST a
 	(requires (fun h0 -> true))
-	(ensures (fun h0 v h1 -> 
-	  modifies loc_none h0 h1 /\ r_inv h1 v /\
-	  region_of v = r /\ MHS.fresh_region r h0 h1 /\
+	(ensures (fun h0 v h1 ->
+	  Set.equal (Map.domain (HS.get_hmap h1))
+	  	    (Map.domain (HS.get_hmap h0)) /\
+	  modifies loc_none h0 h1 /\ 
+	  r_inv h1 v /\ region_of v = r /\
 	  r_repr h1 v == Ghost.reveal irepr))) ->
 
     // Destruction
@@ -109,37 +111,55 @@ type rvector #a (rg:regional a) = V.vector a
 
 /// The invariant for each element
 
-val elems_inv:
-  #a:Type0 -> #rg:regional a ->
-  h:HS.mem -> rv:rvector rg -> 
-  i:uint32_t -> j:uint32_t{i <= j && j <= V.size_of rv} ->
+val rs_elems_inv:
+  #a:Type0 -> rg:regional a ->
+  h:HS.mem -> rs:S.seq a -> 
+  i:nat -> j:nat{i <= j && j <= S.length rs} ->
   GTot Type0
-let elems_inv #a #rg h rv i j =
-  V.forall_ h rv i j (Rgl?.r_inv rg h)
+let rs_elems_inv #a rg h rs i j =
+  V.forall_seq rs i j (Rgl?.r_inv rg h)
 
 val rv_elems_inv:
-  #a:Type0 -> #rg:regional a ->
-  h:HS.mem -> rv:rvector rg -> GTot Type0
-let rv_elems_inv #a #rg h rv =
-  elems_inv h rv 0ul (V.size_of rv)
-
-val elems_reg:
   #a:Type0 -> #rg:regional a ->
   h:HS.mem -> rv:rvector rg ->
   i:uint32_t -> j:uint32_t{i <= j && j <= V.size_of rv} ->
   GTot Type0
-let elems_reg #a #rg h rv i j =
-  V.forall_ h rv i j
-    (fun v -> HH.extends (Rgl?.region_of rg v) (V.frameOf rv)) /\
-  V.forall2 h rv i j
+let rv_elems_inv #a #rg h rv i j =
+  rs_elems_inv rg h (V.as_seq h rv) (U32.v i) (U32.v j) 
+
+val elems_inv:
+  #a:Type0 -> #rg:regional a ->
+  h:HS.mem -> rv:rvector rg ->
+  GTot Type0
+let elems_inv #a #rg h rv =
+  rv_elems_inv h rv 0ul (V.size_of rv)
+
+val rs_elems_reg:
+  #a:Type0 -> rg:regional a ->
+  rs:S.seq a -> prid:HH.rid ->
+  i:nat -> j:nat{i <= j && j <= S.length rs} ->
+  GTot Type0
+let rs_elems_reg #a rg rs prid i j =
+  V.forall_seq rs i j
+    (fun v -> HH.extends (Rgl?.region_of rg v) prid) /\
+  V.forall2_seq rs i j
     (fun v1 v2 -> HH.disjoint (Rgl?.region_of rg v1)
 			      (Rgl?.region_of rg v2))
 
 val rv_elems_reg:
   #a:Type0 -> #rg:regional a ->
-  h:HS.mem -> rv:rvector rg -> GTot Type0
-let rv_elems_reg #a #rg h rv =
-  elems_reg h rv 0ul (V.size_of rv)
+  h:HS.mem -> rv:rvector rg -> 
+  i:uint32_t -> j:uint32_t{i <= j && j <= V.size_of rv} ->
+  GTot Type0
+let rv_elems_reg #a #rg h rv i j =
+  rs_elems_reg rg (V.as_seq h rv) (V.frameOf rv) (U32.v i) (U32.v j)
+
+val elems_reg:
+  #a:Type0 -> #rg:regional a ->
+  h:HS.mem -> rv:rvector rg ->
+  GTot Type0
+let elems_reg #a #rg h rv =
+  rv_elems_reg h rv 0ul (V.size_of rv)
 
 /// The invariant of rvector
 
@@ -154,30 +174,36 @@ val rv_inv:
   #a:Type0 -> #rg:regional a ->
   h:HS.mem -> rv:rvector rg -> GTot Type0
 let rv_inv #a #rg h rv =
-  rv_elems_inv h rv /\
-  rv_elems_reg h rv /\
+  elems_inv h rv /\
+  elems_reg h rv /\
   rv_itself_inv h rv
 
 /// Fine-grained control of regions (frames)
 
-private val rv_loc_elem:
-  #a:Type0 -> #rg:regional a ->
-  h:HS.mem -> rv:rvector rg ->
-  i:uint32_t{i < V.size_of rv} ->
+private val rs_loc_elem:
+  #a:Type0 -> rg:regional a ->
+  rs:S.seq a -> i:nat{i < S.length rs} ->
   GTot loc
-private let rv_loc_elem #a #rg h rv i =
+private let rs_loc_elem #a rg rs i =
   B.loc_all_regions_from false 
-    (Rgl?.region_of rg (S.index (V.as_seq h rv) (U32.v i)))
+    (Rgl?.region_of rg (S.index rs i))
+
+private val rs_loc_elems:
+  #a:Type0 -> rg:regional a ->
+  rs:S.seq a -> i:nat -> j:nat{i <= j && j <= S.length rs} -> 
+  GTot loc (decreases j)
+private let rec rs_loc_elems #a rg rs i j =
+  if i = j then loc_none
+  else loc_union (rs_loc_elems rg rs i (j - 1))
+		 (rs_loc_elem rg rs (j - 1))
 
 private val rv_loc_elems:
   #a:Type0 -> #rg:regional a ->
   h:HS.mem -> rv:rvector rg ->
   i:uint32_t -> j:uint32_t{i <= j && j <= V.size_of rv} -> 
-  GTot loc (decreases (U32.v j))
-private let rec rv_loc_elems #a #rg h rv i j =
-  if i = j then loc_none
-  else loc_union (rv_loc_elems h rv i (j - 1ul))
-		 (rv_loc_elem h rv (j - 1ul))
+  GTot loc
+private let rv_loc_elems #a #rg h rv i j =
+  rs_loc_elems rg (V.as_seq h rv) (U32.v i) (U32.v j)
 
 // Inclusion
 
@@ -190,61 +216,83 @@ let loc_all_exts_from preserve_liveness r =
       (HS.mod_set (Set.singleton r))
       (Set.complement (Set.singleton r)))
 
-private val rv_loc_elem_included:
-  #a:Type0 -> #rg:regional a ->
-  h:HS.mem -> rv:rvector rg ->
-  i:uint32_t{i < V.size_of rv} ->
-  Lemma (requires (HH.extends (Rgl?.region_of rg (V.get h rv i))
-			      (V.frameOf rv)))
-	(ensures (loc_includes (loc_all_exts_from false (V.frameOf rv))
-  			       (rv_loc_elem h rv i)))
-private let rv_loc_elem_included #a #rg h rv i = ()
+private val rs_loc_elem_included:
+  #a:Type0 -> rg:regional a ->
+  rs:S.seq a -> prid:HH.rid ->
+  i:nat{i < S.length rs} ->
+  Lemma (requires (HH.extends (Rgl?.region_of rg (S.index rs i)) prid))
+	(ensures (loc_includes (loc_all_exts_from false prid)
+  			       (rs_loc_elem rg rs i)))
+private let rs_loc_elem_included #a rg rs prid i = ()
+
+private val rs_loc_elems_included:
+  #a:Type0 -> rg:regional a ->
+  rs:S.seq a -> prid:HH.rid ->
+  i:nat -> j:nat{i <= j && j <= S.length rs} -> 
+  Lemma (requires (rs_elems_reg rg rs prid i j))
+	(ensures (loc_includes (loc_all_exts_from false prid)
+  			       (rs_loc_elems rg rs i j)))
+	(decreases j)
+private let rec rs_loc_elems_included #a rg rs prid i j =
+  if i = j then ()
+  else (rs_loc_elem_included rg rs prid (j - 1);
+       rs_loc_elems_included rg rs prid i (j - 1))
 
 private val rv_loc_elems_included:
   #a:Type0 -> #rg:regional a ->
   h:HS.mem -> rv:rvector rg ->
-  i:uint32_t -> j:uint32_t{i <= j && j <= V.size_of rv} -> 
-  Lemma (requires (elems_reg h rv i j))
+  i:uint32_t -> j:uint32_t{i <= j && j <= V.size_of rv} ->
+  Lemma (requires (rv_elems_reg h rv i j))
 	(ensures (loc_includes (loc_all_exts_from false (V.frameOf rv))
   			       (rv_loc_elems h rv i j)))
-	(decreases (U32.v j))
-private let rec rv_loc_elems_included #a #rg h rv i j =
-  if i = j then ()
-  else (rv_loc_elem_included h rv (j - 1ul);
-       rv_loc_elems_included h rv i (j - 1ul))
+private let rv_loc_elems_included #a #rg h rv i j =
+  rs_loc_elems_included rg (V.as_seq h rv) (V.frameOf rv) (U32.v i) (U32.v j)
 
 // Disjointness
 
-private val rv_loc_elem_disj:
-  #a:Type0 -> #rg:regional a ->
-  h:HS.mem -> rv:rvector rg ->
-  i:uint32_t -> j:uint32_t{i <= j && j <= V.size_of rv} -> 
-  k:uint32_t{i <= k && k < j} ->
-  l:uint32_t{i <= l && l < j && k <> l} ->
-  Lemma (requires (elems_reg h rv i j))
-	(ensures (loc_disjoint (rv_loc_elem h rv k)
-			       (rv_loc_elem h rv l)))
-private let rv_loc_elem_disj #a #rg h rv i j k l =
-  V.forall2_seq_ok
-    (V.as_seq h rv) (U32.v i) (U32.v j) (U32.v k) (U32.v l)
-    (fun v1 v2 -> HH.disjoint (Rgl?.region_of rg v1)
-  			      (Rgl?.region_of rg v2))
+private val rs_loc_elem_disj:
+  #a:Type0 -> rg:regional a ->
+  rs:S.seq a -> prid:HH.rid ->
+  i:nat -> j:nat{i <= j && j <= S.length rs} -> 
+  k:nat{i <= k && k < j} ->
+  l:nat{i <= l && l < j && k <> l} ->
+  Lemma (requires (rs_elems_reg rg rs prid i j))
+	(ensures (loc_disjoint (rs_loc_elem rg rs k)
+			       (rs_loc_elem rg rs l)))
+private let rs_loc_elem_disj #a rg rs prid i j k l = ()
 
-private val rv_loc_elems_elem_disj:
-  #a:Type0 -> #rg:regional a ->
-  h:HS.mem -> rv:rvector rg ->
-  i:uint32_t -> j:uint32_t{i <= j && j <= V.size_of rv} -> 
-  k1:uint32_t{i <= k1} ->
-  k2:uint32_t{k1 <= k2 && k2 < j} ->
-  l:uint32_t{i <= l && l < j && (l < k1 || k2 <= l)} ->
-  Lemma (requires (elems_reg h rv i j))
-	(ensures (loc_disjoint (rv_loc_elems h rv k1 k2)
-			       (rv_loc_elem h rv l)))
-	(decreases (U32.v k2))
-private let rec rv_loc_elems_elem_disj #a #rg h rv i j k1 k2 l =
+private val rs_loc_elems_elem_disj:
+  #a:Type0 -> rg:regional a ->
+  rs:S.seq a -> prid:HH.rid ->
+  i:nat -> j:nat{i <= j && j <= S.length rs} -> 
+  k1:nat{i <= k1} ->
+  k2:nat{k1 <= k2 && k2 < j} ->
+  l:nat{i <= l && l < j && (l < k1 || k2 <= l)} ->
+  Lemma (requires (rs_elems_reg rg rs prid i j))
+	(ensures (loc_disjoint (rs_loc_elems rg rs k1 k2)
+			       (rs_loc_elem rg rs l)))
+	(decreases k2)
+private let rec rs_loc_elems_elem_disj #a rg rs prid i j k1 k2 l =
   if k1 = k2 then ()
-  else (rv_loc_elem_disj h rv i j (k2 - 1ul) l;
-       rv_loc_elems_elem_disj h rv i j k1 (k2 - 1ul) l)
+  else (rs_loc_elem_disj rg rs prid i j (k2 - 1) l;
+       rs_loc_elems_elem_disj rg rs prid i j k1 (k2 - 1) l)
+
+private val rs_loc_elems_disj:
+  #a:Type0 -> rg:regional a ->
+  rs:S.seq a -> prid:HH.rid ->
+  i:nat -> j:nat{i <= j && j <= S.length rs} -> 
+  k1:nat{i <= k1} ->
+  k2:nat{k1 <= k2 && k2 < j} ->
+  l1:nat{i <= l1} ->
+  l2:nat{l1 <= l2 && l2 < j} ->
+  Lemma (requires (rs_elems_reg rg rs prid i j /\ (k2 <= l1 || l2 <= k1)))
+	(ensures (loc_disjoint (rs_loc_elems rg rs k1 k2)
+			       (rs_loc_elems rg rs l1 l2)))
+	(decreases k2)
+private let rec rs_loc_elems_disj #a rg rs prid i j k1 k2 l1 l2 =
+  if k1 = k2 then ()
+  else (rs_loc_elems_elem_disj rg rs prid i j l1 l2 (k2 - 1);
+       rs_loc_elems_disj rg rs prid i j k1 (k2 - 1) l1 l2)
 
 private val rv_loc_elems_disj:
   #a:Type0 -> #rg:regional a ->
@@ -254,70 +302,55 @@ private val rv_loc_elems_disj:
   k2:uint32_t{k1 <= k2 && k2 < j} ->
   l1:uint32_t{i <= l1} ->
   l2:uint32_t{l1 <= l2 && l2 < j} ->
-  Lemma (requires (elems_reg h rv i j /\ (k2 <= l1 || l2 <= k1)))
+  Lemma (requires (rv_elems_reg h rv i j /\ (k2 <= l1 || l2 <= k1)))
 	(ensures (loc_disjoint (rv_loc_elems h rv k1 k2)
 			       (rv_loc_elems h rv l1 l2)))
-	(decreases (U32.v k2))
-private let rec rv_loc_elems_disj #a #rg h rv i j k1 k2 l1 l2 =
-  if k1 = k2 then ()
-  else (rv_loc_elems_elem_disj h rv i j l1 l2 (k2 - 1ul);
-       rv_loc_elems_disj h rv i j k1 (k2 - 1ul) l1 l2)
+private let rv_loc_elems_disj #a #rg h rv i j k1 k2 l1 l2 =
+  rs_loc_elems_disj rg (V.as_seq h rv) (V.frameOf rv)
+    (U32.v i) (U32.v j) (U32.v k1) (U32.v k2) (U32.v l1) (U32.v l2)
 
 // Preservation based on disjointness
-
-private val rv_loc_elem_preserved:
-  #a:Type0 -> #rg:regional a -> rv:rvector rg -> 
-  i:uint32_t{i < V.size_of rv} ->
-  p:loc -> h0:HS.mem -> h1:HS.mem ->
-  Lemma (requires (loc_disjoint p (V.loc_vector_within rv i (i + 1ul)) /\
-		  modifies p h0 h1))
-	(ensures (rv_loc_elem h0 rv i == rv_loc_elem h1 rv i))
-private let rv_loc_elem_preserved #a #rg rv i p h0 h1 =
-  // Requires a more general version of `V.get_preserved`
-  assume (V.get h0 rv i == V.get h1 rv i)
 
 private val rv_loc_elems_preserved:
   #a:Type0 -> #rg:regional a -> rv:rvector rg -> 
   i:uint32_t -> j:uint32_t{i <= j && j < V.size_of rv} ->
   p:loc -> h0:HS.mem -> h1:HS.mem ->
-  Lemma (requires (loc_disjoint p (V.loc_vector_within rv i j) /\
+  Lemma (requires (V.live h0 rv /\
+		  // loc_disjoint p (V.loc_vector_within rv i j) /\
+		  loc_disjoint p (V.loc_vector rv) /\
 		  modifies p h0 h1))
 	(ensures (rv_loc_elems h0 rv i j ==
 		 rv_loc_elems h1 rv i j))
 	(decreases (U32.v j))
-private let rec rv_loc_elems_preserved #a #rg rv i j p h0 h1 =
-  if i = j then ()
-  else (rv_loc_elem_preserved rv (j - 1ul) p h0 h1;
-       rv_loc_elems_preserved rv i (j - 1ul) p h0 h1)
+private let rv_loc_elems_preserved #a #rg rv i j p h0 h1 = ()
 
-private val elem_inv_preserved:
-  #a:Type0 -> #rg:regional a -> rv:rvector rg -> 
-  i:uint32_t{i < V.size_of rv} ->
+private val rs_elems_inv_preserved:
+  #a:Type0 -> rg:regional a -> rs:S.seq a -> 
+  i:nat -> j:nat{i <= j && j <= S.length rs} ->
   p:loc -> h0:HS.mem -> h1:HS.mem ->
-  Lemma (requires (Rgl?.r_inv rg h0 (V.get h0 rv i) /\
-		  loc_disjoint p (V.loc_vector_within rv i (i + 1ul)) /\
-		  loc_disjoint p (rv_loc_elem h0 rv i) /\
+  Lemma (requires (rs_elems_inv rg h0 rs i j /\
+		  loc_disjoint p (rs_loc_elems rg rs i j) /\
 		  modifies p h0 h1))
-	(ensures (Rgl?.r_inv rg h1 (V.get h1 rv i)))
-private let elem_inv_preserved #a #rg rv i p h0 h1 =
-  // Requires a more general version of `V.get_preserved`
-  assume (V.get h0 rv i == V.get h1 rv i);
-  Rgl?.r_sep rg (V.get h0 rv i) p h0 h1
+	(ensures (rs_elems_inv rg h1 rs i j))
+	(decreases j)
+private let rec rs_elems_inv_preserved #a rg rs i j p h0 h1 =
+  if i = j then ()
+  else (rs_elems_inv_preserved rg rs i (j - 1) p h0 h1;
+       Rgl?.r_sep rg (S.index rs (j - 1)) p h0 h1)
 
-private val elems_inv_preserved:
+private val rv_elems_inv_preserved:
   #a:Type0 -> #rg:regional a -> rv:rvector rg -> 
   i:uint32_t -> j:uint32_t{i <= j && j <= V.size_of rv} ->
   p:loc -> h0:HS.mem -> h1:HS.mem ->
-  Lemma (requires (elems_inv h0 rv i j /\
-		  loc_disjoint p (V.loc_vector_within rv i j) /\
+  Lemma (requires (V.live h0 rv /\
+		  rv_elems_inv h0 rv i j /\
+		  // loc_disjoint p (V.loc_vector_within rv i j) /\
+		  loc_disjoint p (V.loc_vector rv) /\
 		  loc_disjoint p (rv_loc_elems h0 rv i j) /\
 		  modifies p h0 h1))
-	(ensures (elems_inv h1 rv i j))
-	(decreases (U32.v j))
-private let rec elems_inv_preserved #a #rg rv i j p h0 h1 =
-  if i = j then ()
-  else (elems_inv_preserved rv i (j - 1ul) p h0 h1;
-       elem_inv_preserved rv (j - 1ul) p h0 h1)
+	(ensures (rv_elems_inv h1 rv i j))
+private let rv_elems_inv_preserved #a #rg rv i j p h0 h1 =
+  rs_elems_inv_preserved rg (V.as_seq h0 rv) (U32.v i) (U32.v j) p h0 h1
 
 /// Representation
 
@@ -356,15 +389,15 @@ val as_seq_sub_as_seq:
 	[SMTPat (as_seq_sub h rv 0ul (V.size_of rv))]
 let as_seq_sub_as_seq #a #rg h rv = ()
 
-val as_seq_seq_upd:
-  #a:Type0 -> #rg:regional a -> 
-  h:HS.mem -> rs:S.seq a ->
-  i:nat -> j:nat{i <= j && j <= S.length rs} ->
-  k:nat{i <= k && k < j} -> v:a ->
-  Lemma (S.equal (as_seq_seq h (S.upd rs k v) i j)
-		 (S.upd (as_seq_seq h rs i j) (k - i) (Rgl?.r_repr rg h v)))
-let as_seq_seq_upd #a #rg h rs i j k v =
-  admit ()
+// val as_seq_seq_upd:
+//   #a:Type0 -> #rg:regional a -> 
+//   h:HS.mem -> rs:S.seq a ->
+//   i:nat -> j:nat{i <= j && j <= S.length rs} ->
+//   k:nat{i <= k && k < j} -> v:a ->
+//   Lemma (S.equal (as_seq_seq h (S.upd rs k v) i j)
+// 		 (S.upd (as_seq_seq h rs i j) (k - i) (Rgl?.r_repr rg h v)))
+// let as_seq_seq_upd #a #rg h rs i j k v =
+//   admit ()
 
 // Preservation based on disjointness
 
@@ -377,7 +410,6 @@ let as_seq_seq_upd #a #rg h rs i j k v =
   // loc_disjoint p (loc_all_exts_from
   // 		  modifies p h0 h1))
   // 	(ensures (rv_loc_elem h0 rv i == rv_loc_elem h1 rv i))
-  
 
 // val vec_as_seq_eq_rv_inv:
 //   #a:Type0 -> #rg:regional a -> 
@@ -407,15 +439,18 @@ private val create_:
     (ensures (fun h0 _ h1 ->
       modifies (V.loc_vector_within rv 0ul cidx) h0 h1 /\
       rv_itself_inv h1 rv /\
-      elems_inv h1 rv 0ul cidx /\
-      elems_reg h1 rv 0ul cidx /\
+      rv_elems_inv h1 rv 0ul cidx /\
+      rv_elems_reg h1 rv 0ul cidx /\
       S.equal (as_seq_sub h1 rv 0ul cidx)
       	      (S.create (U32.v cidx) (Ghost.reveal (Rgl?.irepr rg))) /\
       // the loop invariant for this function
       V.forall_ h1 rv 0ul cidx
-	(fun r -> MHS.fresh_region (Rgl?.region_of rg r) h0 h1)))
+	(fun r -> MHS.fresh_region (Rgl?.region_of rg r) h0 h1) /\
+      Set.subset (Map.domain (MHS.get_hmap h0))
+		 (Map.domain (MHS.get_hmap h1))))
     (decreases (U32.v cidx))
 private let rec create_ #a #rg rv cidx =
+  let hh0 = HST.get () in
   if cidx = 0ul then ()
   else (let nrid = new_region_ (V.frameOf rv) in
        let r_init = Rgl?.r_init rg in
@@ -425,6 +460,7 @@ private let rec create_ #a #rg rv cidx =
        V.assign rv (cidx - 1ul) v;
 
        let hh2 = HST.get () in
+
        Rgl?.r_sep
 	 rg (V.get hh2 rv (cidx - 1ul))
 	 (V.loc_vector_within rv (cidx - 1ul) cidx)
@@ -436,12 +472,9 @@ private let rec create_ #a #rg rv cidx =
 	 rg (V.get hh3 rv (cidx - 1ul))
 	 (V.loc_vector_within rv 0ul (cidx - 1ul))
 	 hh2 hh3;
-       elem_inv_preserved 
-       	 rv (cidx - 1ul) (V.loc_vector_within rv 0ul (cidx - 1ul))
-       	 hh2 hh3;
        V.forall2_extend hh3 rv 0ul (cidx - 1ul)
-	 (fun r1 r2 -> HH.disjoint (Rgl?.region_of rg r1)
-				   (Rgl?.region_of rg r2)))
+       	 (fun r1 r2 -> HH.disjoint (Rgl?.region_of rg r1)
+       				   (Rgl?.region_of rg r2)))
 
 val create_rid:
   #a:Type0 -> rg:regional a ->
@@ -594,13 +627,13 @@ let assign #a #rg rv i v =
   assert (S.equal (as_seq hh1 rv)
 		  (as_seq_seq hh1 (S.upd (V.as_seq hh0 rv) (U32.v i) v)
 			      0 (U32.v (V.size_of rv))));
-  as_seq_seq_upd #a #rg
-    hh1 (V.as_seq hh0 rv) 0 (U32.v (V.size_of rv))
-    (U32.v i) v;
-  assert (S.equal (as_seq hh1 rv)
-  		  (S.upd (as_seq_seq hh1 (V.as_seq hh0 rv)
-  				     0 (U32.v (V.size_of rv)))
-  			 (U32.v i) (Rgl?.r_repr rg hh0 v)));
+  // as_seq_seq_upd #a #rg
+  //   hh1 (V.as_seq hh0 rv) 0 (U32.v (V.size_of rv))
+  //   (U32.v i) v;
+  // assert (S.equal (as_seq hh1 rv)
+  // 		  (S.upd (as_seq_seq hh1 (V.as_seq hh0 rv)
+  // 				     0 (U32.v (V.size_of rv)))
+  // 			 (U32.v i) (Rgl?.r_repr rg hh0 v)));
   admit ()
 
 val assign_copy:
@@ -626,8 +659,8 @@ val free_elems:
   HST.ST unit
     (requires (fun h0 -> 
       V.live h0 rv /\
-      elems_inv h0 rv 0ul (idx + 1ul) /\
-      elems_reg h0 rv 0ul (idx + 1ul)))
+      rv_elems_inv h0 rv 0ul (idx + 1ul) /\
+      rv_elems_reg h0 rv 0ul (idx + 1ul)))
     (ensures (fun h0 _ h1 ->
       modifies (rv_loc_elems h0 rv 0ul (idx + 1ul)) h0 h1))
 let rec free_elems #a #rg rv idx =
@@ -636,11 +669,11 @@ let rec free_elems #a #rg rv idx =
   r_free (V.index rv idx);
 
   let hh1 = HST.get () in
-  rv_loc_elems_elem_disj hh0 rv 0ul (idx + 1ul) 0ul idx idx;
-  elems_inv_preserved 
-    rv 0ul idx (rv_loc_elem hh0 rv idx) hh0 hh1;
-  rv_loc_elems_preserved
-    rv 0ul idx (rv_loc_elem hh0 rv idx) hh0 hh1;
+  rs_loc_elems_elem_disj
+    rg (V.as_seq hh0 rv) (V.frameOf rv)
+    0 (U32.v idx + 1) 0 (U32.v idx) (U32.v idx);
+  rv_elems_inv_preserved 
+    rv 0ul idx (rs_loc_elem rg (V.as_seq hh0 rv) (U32.v idx)) hh0 hh1;
 
   if idx <> 0ul then
     free_elems rv (idx - 1ul)
